new language features: Cut, Subgoal, User < >. prettier efficient proof scripts.
Cut limits non-determinism by pruning.
Subgoal implements subgoal focusing.
User < > allows us to utilise methods defined by users using Eisbach.

User < > is still in the experimental stage.
See their use cases in Example.thy.

The style of generated proof scripts are changed.
Now, PSL prints "defer" instead of "apply(tactic {* defer_tac 1 *})".

Monadic_Interpreter is refactored.

Example.thy
@@ -1,10 +1,56 @@
 (* This file, Example.thy, contains small examples, including Example2 presented in the FM2016 draft. *)
 theory Example
-imports PSL 
+imports PSL "~~/src/HOL/Eisbach/Eisbach"
 begin
 
-strategy pang_str = Thens [Dynamic (Rule), Dynamic (Rule), Dynamic (ERule)]
-lemma "(A = True) = A"
+method my_simp = simp
+
+strategy UserSimp = User< my_simp >
+lemma "True \<and> True \<or> False"
+find_proof UserSimp
+oops
+
+method test_match =(match premises in I: "Q \<longrightarrow> A" and I':"Q" for Q A \<Rightarrow>
+   \<open>match conclusion in A \<Rightarrow> \<open>rule mp [OF I I']\<close>\<close>)
+
+lemma "\<And> P. Q \<longrightarrow> P \<Longrightarrow> Q \<Longrightarrow> P"
+by (match premises in I: "Q \<longrightarrow> A" and I':"Q" for A \<Rightarrow>
+   \<open>match conclusion in A \<Rightarrow> \<open>rule mp [OF I I']\<close>\<close>)
+
+method if_match = (match conclusion in "((P::'a \<Rightarrow> 'b) = (Q::'a \<Rightarrow> 'b))" for P Q \<Rightarrow> \<open>succeed\<close>)
+method extI =  (rule ext)
+method if_match2 = (match conclusion in "((P::'a) = (Q::'a))" for P Q \<Rightarrow> \<open>succeed\<close>)
+
+strategy IfMatch  = Thens [User <if_match>, Skip]
+strategy IfMatch2 = Thens [User <if_match>, User <succeed>]
+strategy IfMatch3 = Thens [User <if_match>, Rule]
+strategy IfMatch4 = Thens [User <if_match>, User < rule >]
+strategy IfMatch5 = Thens [Skip, User <succeed>]
+strategy IfMatch6 = Thens [Skip, User < if_match >, Skip]
+strategy IfMatch7 = Thens [User <succeed>, Skip]
+strategy IfMatch8 = Alts [User <succeed>, User <succeed>]
+
+consts "QQ"::"'a \<Rightarrow> 'b"
+consts "PP"::"'a \<Rightarrow> 'b"
+
+lemma "(QQ = PP)"
+find_proof IfMatch
+find_proof IfMatch2
+find_proof IfMatch3
+find_proof IfMatch4
+find_proof IfMatch5
+find_proof IfMatch6
+find_proof IfMatch7
+find_proof IfMatch8
+apply(if_match)
+oops
+
+definition "my_foo \<equiv> True"
+thm my_foo_def(1)
+
+strategy UserSimp2 = Thens [User < simp add: my_foo_def(1) >, IsSolved]
+lemma "my_foo"
+find_proof UserSimp2
 oops
 
 strategy Hammer = Hammer
@@ -26,6 +72,18 @@ lemma
  assumes "P"
  shows "P"
 find_proof FFpaltHam
+oops
+
+strategy MultiFF = Thens [Fastforce, IsSolved, Fastforce, IsSolved]
+lemma "True" and "True"
+apply -
+subgoal
+find_proof MultiFF
+oops
+
+strategy Auto2 = Thens [Subgoal, Auto, IsSolved, Subgoal, Auto, IsSolved]
+lemma "True" and "True"
+find_proof Auto2
 oops
 
 inductive foo::"'a \<Rightarrow> 'a \<Rightarrow> bool" where
@@ -81,11 +139,22 @@ shows 1:"ps_safe p s"
  and  2:"valid_trans p s s' x"
  and  3:"ps_safe p s'"
 find_proof Hammers
+apply -
 oops
 
 lemma "x \<or> True" and "(1::int) > 0"
 try_hard
 apply -
 oops
+
+strategy testCut = Thens [Repeat (Cut 10 (Dynamic (Rule))), IsSolved]
+lemma "True \<and> True"
+find_proof testCut
+oops
+
+lemma "True \<equiv> True"
+thm meta_eq_to_obj_eq
+find_theorems "?x \<equiv> ?y" "?x = ?y" name:"meta"
+apply auto done
 
 end
