PSL.thy
@@ -5,4 +5,10 @@ theory PSL
 imports "PSLCore/Try_Hard"
 begin
 
+text{* Uncomment the following to unleash the power parallelism. *}
+(*
+ML {* Multithreading.max_threads_update 28 *}
+ML {* Goal.parallel_proofs := 1 *}
+*)
+
 end
