PSLCore/Monadic_Interpreter_Params.thy
@@ -33,87 +33,103 @@ end;
 
 ML{* structure Monadic_Interpreter_Params : MONADIC_INTERPRETER_PARAMS =
 struct
-
-  open Monadic_Interpreter;
+  open Monadic_Interpreter_Core;
+  structure DU         = Dynamic_Utils;
   type state           = Proof.state;
   type 'a seq          = 'a Seq.seq;
   type ctxt            = Proof.context;
   type thms            = thm list;
   type strings         = string list;
-  type eval_prim       = prim_str -> state stttac;
-  type eval_para       = para_str -> state -> state stttac Seq.seq;
-  type eval_strategic  = atom_strategic * state stttac list -> state stttac;
+  type eval_prim       = cstatic -> state stttac;
+  type eval_para       = cprim_str -> state -> state stttac Seq.seq;
+  type eval_strategic  = cstrategic * state stttac list -> state stttac;
   type m_equal         = state monad -> state monad -> bool;
-  type iddfc           = int -> (atom_str -> state stttac) -> (atom_str -> state stttac);
-  (* For eval_prim. *)
-  val quickcheck_tac   = Quickcheck_Tactic.nontac;
-  val nitpick_tac      = Nitpick_Tactic.nontac;
-  val string_to_stttac = Dynamic_Utils.string_to_stttac_on_pstate;
-  val is_solved        = Tactic.is_solved;
+  type iddfc           = int -> (catom_str -> state stttac) -> (catom_str -> state stttac);
   type log             = Dynamic_Utils.log;
-
   (* do_trace and show_trace are for debugging only. *)
   val do_trace = false;
   fun show_trace text = if do_trace then tracing text else ();
 
+  local
+  structure User_Seed : DYNAMIC_TACTIC_GENERATOR_SEED =
+  struct
+    type modifier  = string;
+    type modifiers = string list;
+    fun get_all_modifiers _ = [];
+    fun mods_to_string mods = String.concatWith " " mods;
+  end;
+  structure User_Tactic_Generator : DYNAMIC_TACTIC_GENERATOR =
+    mk_Dynamic_Tactic_Generator (User_Seed);
+  in
+  fun user_stttac (meth:string) =
+    User_Tactic_Generator.meth_name_n_modifiers_to_stttac_on_state meth [(* ignores log *)];
+  end;
+
   (* I cannot move the definition of "eval_prim" into mk_Monadic_Interpreter,
    * because its type signature is too specific.*)
-  fun eval_prim (prim:prim_str) (goal_state:state) =
+  fun eval_prim (prim:cstatic) (goal_state:state) =
     let
-      val defer_meth_name        = "tactic {* defer_tac 1 *" ^"}";
-      val defer_stttac           = Seq.single o (Proof.defer 1);
-      val log_n_nontac_to_stttac = Dynamic_Utils.log_n_nontac_to_stttac;
-      val tac_on_proof_state : state stttac =
-       case prim of
-        CClarsimp =>     (show_trace "CClarsimp";      string_to_stttac "clarsimp")
-      | CSimp =>         (show_trace "CSimp";          string_to_stttac "simp")
-      | CFastforce =>    (show_trace "CFastforce";     string_to_stttac "fastforce")
-      | CAuto =>         (show_trace "CAuto";          string_to_stttac "auto")
-      | CInduct =>       (show_trace "CInduct";        string_to_stttac "induct")
-      | CCoinduction =>  (show_trace "CCoinduct";      string_to_stttac "coinduction")
-      | CCases  =>       (show_trace "CCases";         string_to_stttac "cases")
-      | CRule   =>       (show_trace "CRule";          string_to_stttac "rule")
-      | CErule  =>       (show_trace "CErule";         string_to_stttac "erule")
-      | CIntroClasses => (show_trace "CIntro_Classes"; string_to_stttac "intro_classes")
-      | CTransfer =>     (show_trace "CTransfer";      string_to_stttac "transfer")
-      | CNormalization =>(show_trace "CNormalization"; string_to_stttac "normalization")
-      | CHammer =>       (show_trace "CHammer";        Dynamic_Sledgehammer.pstate_stttacs)
-      (* assertion tactics *)
-      | CIsSolved =>     (show_trace "CIs_Solved";     log_n_nontac_to_stttac ([], is_solved))
-      | CQuickcheck=>    (show_trace "CQuickcheck";    log_n_nontac_to_stttac ([], quickcheck_tac))
-      | CNitpick   =>    (show_trace "CNitpick";       log_n_nontac_to_stttac ([], nitpick_tac))
-      | CDefer     =>    (show_trace "CDefer";
-          log_n_nontac_to_stttac ([{methN = defer_meth_name, using = [], back = 0}], defer_stttac))
+      (* For eval_prim. *)
+      val quickcheck_tac   = Quickcheck_Tactic.nontac;
+      val nitpick_tac      = Nitpick_Tactic.nontac;
+      val string_to_stttac = Dynamic_Utils.string_to_stttac_on_pstate;
+      val is_solved        = Tactic.is_solved;
+      val single           = Seq.single;
+      val defer_tac        = single o (Proof.defer 1);
+      val subgoal_tac      = single o #2 o Subgoal.subgoal Attrib.empty_binding NONE (false, []);
+      val to_stttac        = Dynamic_Utils.log_n_nontac_to_stttac;
+      val tac_on_proof_state : state stttac = case prim of
+        CPrim CClarsimp =>     (show_trace "CClarsimp";      string_to_stttac "clarsimp")
+      | CPrim CSimp =>         (show_trace "CSimp";          string_to_stttac "simp")
+      | CPrim CFastforce =>    (show_trace "CFastforce";     string_to_stttac "fastforce")
+      | CPrim CAuto =>         (show_trace "CAuto";          string_to_stttac "auto")
+      | CPrim CInduct =>       (show_trace "CInduct";        string_to_stttac "induct")
+      | CPrim CCoinduction =>  (show_trace "CCoinduct";      string_to_stttac "coinduction")
+      | CPrim CCases  =>       (show_trace "CCases";         string_to_stttac "cases")
+      | CPrim CRule   =>       (show_trace "CRule";          string_to_stttac "rule")
+      | CPrim CErule  =>       (show_trace "CErule";         string_to_stttac "erule")
+      | CSpec CIntroClasses => (show_trace "CIntro_Classes"; string_to_stttac "intro_classes")
+      | CSpec CTransfer =>     (show_trace "CTransfer";      string_to_stttac "transfer")
+      | CSpec CNormalization =>(show_trace "CNormalization"; string_to_stttac "normalization")
+      | CSpec CSubgoal =>      (show_trace "CSubgoal";       to_stttac ([DU.Subgoal], subgoal_tac))
+      | CSubt CHammer =>       (show_trace "CHammer";        Dynamic_Sledgehammer.pstate_stttacs)
+      | CSpec CIsSolved =>     (show_trace "CIs_Solved";     to_stttac ([DU.Done], is_solved))
+      | CSubt CQuickcheck=>    (show_trace "CQuickcheck";    to_stttac ([], quickcheck_tac))
+      | CSubt CNitpick   =>    (show_trace "CNitpick";       to_stttac ([], nitpick_tac))
+      | CSpec CDefer     =>    (show_trace "CDefer";         to_stttac ([DU.Defer], defer_tac))
+      | CUser tac_name =>      (show_trace tac_name;         user_stttac tac_name);
     in
        tac_on_proof_state goal_state
-          handle THM _ =>  mzero
-               | TERM _ => mzero
-               | Empty =>  mzero
-               | TYPE _ => mzero : state monad
+          handle THM _ =>   mzero
+               | ERROR _ => mzero
+               | TERM _ =>  mzero
+               | Empty =>   mzero
+               | TYPE _ =>  mzero : state monad
     end;
 
-  fun eval_para (str:para_str) (state:Proof.state) =
+  fun eval_para (str:cprim_str) (state:Proof.state) =
     let
       type 'a stttac = 'a Dynamic_Utils.stttac;
       val get_state_stttacs = case str of
-          CParaSimp =>        (show_trace "CPara_Simp";        Dynamic_Simp.get_state_stttacs)
-        | CParaInduct =>      (show_trace "CPara_Induct";      Dynamic_Induct.get_state_stttacs)
-        | CParaCoinduction => (show_trace "CPara_Coinduction"; Dynamic_Coinduction.get_state_stttacs)
-        | CParaCases =>       (show_trace "CPara_Cases";       Dynamic_Cases.get_state_stttacs)
-        | CParaRule =>        (show_trace "CPara_Rule";        Dynamic_Rule.get_state_stttacs)
-        | CParaErule =>       (show_trace "CPara_Erule";       Dynamic_Erule.get_state_stttacs)
-        | CParaFastforce =>   (show_trace "CPara_Fastforce";   Dynamic_Fastforce.get_state_stttacs)
-        | CParaAuto =>        (show_trace "CPara_Auto";        Dynamic_Auto.get_state_stttacs)
-        | CParaClarsimp =>    (show_trace "CPara_Clarsimp";    Dynamic_Clarsimp.get_state_stttacs)
+          CSimp =>        (show_trace "CPara_Simp";        Dynamic_Simp.get_state_stttacs)
+        | CInduct =>      (show_trace "CPara_Induct";      Dynamic_Induct.get_state_stttacs)
+        | CCoinduction => (show_trace "CPara_Coinduction"; Dynamic_Coinduction.get_state_stttacs)
+        | CCases =>       (show_trace "CPara_Cases";       Dynamic_Cases.get_state_stttacs)
+        | CRule =>        (show_trace "CPara_Rule";        Dynamic_Rule.get_state_stttacs)
+        | CErule =>       (show_trace "CPara_Erule";       Dynamic_Erule.get_state_stttacs)
+        | CFastforce =>   (show_trace "CPara_Fastforce";   Dynamic_Fastforce.get_state_stttacs)
+        | CAuto =>        (show_trace "CPara_Auto";        Dynamic_Auto.get_state_stttacs)
+        | CClarsimp =>    (show_trace "CPara_Clarsimp";    Dynamic_Clarsimp.get_state_stttacs)
     in
       (* It is okay to use the type list internally,
        * as long as the overall monadic interpretation framework is instantiated to Seq.seq for 
        * monad with 0 and plus.*)
       get_state_stttacs state
-      handle THM _  => Seq.empty
-           | Empty  => Seq.empty
-           | TERM _ => Seq.empty
-           | TYPE _ => Seq.empty: state stttac Seq.seq
+      handle THM _   => Seq.empty
+           | ERROR _ => Seq.empty
+           | Empty   => Seq.empty
+           | TERM _  => Seq.empty
+           | TYPE _  => Seq.empty: state stttac Seq.seq
     end;
 
   fun m_equal (st_mona1:state monad) (st_mona2:state monad) =
@@ -131,15 +147,16 @@ struct
       are_same_seq (xs_5, ys_5)
     end;
 
-  fun solve_1st_subg (tac : state stttac) (goal:state) (_:log) =
+  fun solve_1st_subg (tac : state stttac) (goal:state) (log:log) =
     let
       val get_thm = Isabelle_Utils.proof_state_to_thm;
       fun same_except_for_fst_prem' x y = Tactic.same_except_for_fst_prem (get_thm x) (get_thm y)
     in
-      tac goal [] |> Seq.filter (fn (_, st')  => same_except_for_fst_prem' goal st') : (log * state) Seq.seq
+      tac goal log
+      |> Seq.filter (fn (_, st')  => same_except_for_fst_prem' goal st'):(log * state) Seq.seq
     end;
 
-  fun repeat_n (tac : state stttac) (goal : state) = (fn (_:log) =>
+  fun repeat_n (tac : state stttac) (goal : state) = (fn (log:log) =>
     let
       fun repeat_n' (0:int) (g:state) = return g
        |  repeat_n' (n:int) (g:state) = if n < 0 then error "" else
@@ -147,13 +164,19 @@ struct
       val subgoal_num = Isabelle_Utils.proof_state_to_thm goal |> Thm.nprems_of;
     in
       (* We have to add 1 because of Isabelle's strange evaluation (parse-twice thingy).*)
-      repeat_n' subgoal_num goal [] : (log * state) Seq.seq
+      repeat_n' subgoal_num goal log : (log * state) Seq.seq
     end) : state monad;
+
+  fun cut (limit:int) (tac:state stttac) (goal:state) = Seq.take limit o tac goal : state monad;
 
   fun eval_strategic (CSolve1, [tac : state stttac])  = solve_1st_subg tac
    |  eval_strategic (CSolve1, _)  = error "eval_strategic failed. M.Solve1 needs exactly one tactic."
    |  eval_strategic (CRepeatN, [tac : state stttac]) = repeat_n tac
    |  eval_strategic (CRepeatN, _) = error "eval_strategic failed. M.RepeatN needs exactly one tactic."
+   |  eval_strategic (CCut lim, [tac : state stttac]) =
+        if lim > 0 then cut lim tac
+        else error "eval_strategic failed. The limit for CCut has to be larger than 0."
+   |  eval_strategic (CCut _, _)   = error "eval strategic failed. M.CCut needs exactly one tactic.";
 
   fun iddfc (limit:int)
     (smt_eval:'atom_str -> 'state stttac) (atac:'atom_str) (goal:'state) (trace:log) =
